\documentclass{article}
\usepackage{amsmath}
\begin{document}

$
% 1
\begin{vmatrix} t = -x^2\\  dt = -2xdx\\ xdx = -\frac{dt}{2} \end{vmatrix}
$

$
% 2
-\frac{1}{2} \int e^t dt
$

$
% 3
-\frac{1}{2}e^t + c
$

$
% 4
-\frac{1}{2}e^{-x^2} + c
$

$
% 1
\begin{vmatrix} t = a^2-x^2\\  dt = -2xdx\\ xdx = -\frac{dt}{2} \end{vmatrix}
$

$
% 2
-\frac{1}{2} \int \sqrt{t} dt
$

$
% 3
-\frac{1}{3} t^{\frac{3}{2}} + c
$

$
% 4
-\frac{1}{3} \sqrt{a^2 - x^2}^3
$

$
% 1
\begin{vmatrix} u = x   &  \frac{dv}{dx} = e^{-x} \\ \frac{du}{dx} = 1   &  v = -e^{-x}\end{vmatrix}
$

$
% 2
-xe^{-x} + \int e^{-x}dx
$

$
% 3
-xe^{-x} - e^{-x} + c
$

$
% 1
\int \frac{sinx}{cosx}dx
$

$
% 2
\begin{vmatrix} t = cosx \\ dt = -sinxdx \end{vmatrix}
$

$
% 3
-\int \frac{1}{t}dt
$

$
% 4
-lnt + c
$

$
% 5
-ln(cosx) + c
$

$
% 1
\begin{vmatrix} t = lnx \\ dt = \frac{1}{x}dx  \end{vmatrix}
$

$
% 2
\int \frac{1}{t}dt
$

$
% 3
lnt + c
$

$
% 4
ln(lnx) + c
$

$
% 1
\begin{vmatrix} u = x   &  \frac{dv}{dx} = sinx \\ \frac{du}{dx} = 1  &   v = -cosx\end{vmatrix}
$

$
% 2
-xcosx + \int cosxdx
$

$
% 3
-xcosx + sinx + c
$


\end{document}