\documentclass{article}
\usepackage{amsmath}

\begin{document}

$
% 1
\begin{vmatrix} t = \sqrt{x}\\  dt = \frac{1}{2\sqrt{x}}dx\\ dx = 2tdt \end{vmatrix}
$

$
% 2
2\int te^t dt 
$

$
% 3
\begin{vmatrix} u = t & \frac{dv}{dt} = e^t\\  \frac{du}{dt} = 1 & v = e^t\end{vmatrix}
$

$
% 4
te^t - \int e^t
$

$
% 5
te^t - e^t + c
$

$
% 6
\sqrt{x}e^{\sqrt{x}} - e^{\sqrt{x}} + c
$

$
% 1
\begin{vmatrix} u = sin(lnx) & \frac{dv}{dt} = 1\\  \frac{du}{dt} = \frac{1}{x}cos(lnx) & v = x \end{vmatrix}
$

$
% 2
xsin(lnx) - \int cos(lnx)dx
$

$
% 3
\begin{vmatrix} u = cos(lnx) & \frac{dv}{dt} = 1\\  \frac{du}{dt} = -\frac{1}{x} sin(lnx) & v = x \end{vmatrix}
$

$
% 4
xsin(lnx) - xcos(lnx) - \int sin(lnx)dx
$

$
% 5
\frac{1}{2}x(sin(lnx) - cos(lnx)) + c
$

$
% 1
\int \frac{cosx}{ln(sinx)sinx}dx 
$

$
% 2
\begin{vmatrix} t = sinx \\ dt = cosxdx  \end{vmatrix}
$

$
% 3
\frac{1}{tlnt}dt
$

$
% 4
\begin{vmatrix} u = lnt \\ du = \frac{1}{t}dt \end{vmatrix}
$

$
% 5
\int \frac{1}{u}du
$

$
% 6
lnu + c
$

$
% 7
ln(ln(sinx)) + c
$

$
% 1
\int \frac{e^x}{e^{2x}+1}dx
$

$
% 2
\begin{vmatrix} t = e^x \\  dt = e^xdx \end{vmatrix}
$

$
% 3
\frac{1}{t^2 + 1}dt
$

$
% 4
arctgt + c
$

$
% 5
arctg(e^x) + c
$

$
% 1
\begin{vmatrix} u = arcsinx & \frac{dv}{dt} = 1 \\  \frac{du}{dt} = \frac{1}{\sqrt{1 - x^2}} & v = x \end{vmatrix}
$

$
% 2
xarcsinx - \int \frac{x}{\sqrt{1-x^2}}
$

$
% 3
\begin{vmatrix} t = 1 - x^2 \\ dt = -2xdx \\ -\frac{1}{2}dt = xdx \end{vmatrix}
$

$
% 4
xarcsinx + \int \frac{1}{2\sqrt{t}}dt
$

$
% 5
xarcsinx + \sqrt{t} + c
$

$
% 6
xarcsinx + \sqrt{1-x^2} + c
$

$
% 1
\int \frac{1}{2}(1-cos2x)\cdot\frac{1}{2}(1+cos2x)dx
$

$
% 2
\frac{1}{4}(1 - cos^2 2x)dx
$

$
% 3
\frac{1}{4} \int sin^2 2xdx 
$

$
% 4
\frac{1}{8} \int (1 - cos4x)dx 
$

$
% 5
\frac{1}{8}x + \frac{1}{32}sin4x + c
$





\end{document}